new file:   c/tlpi/catch_rtsigs.c 	new file:   c/tlpi/t_sigqueue.c 	new file:   c/tlpi/t_sigsuspend.c 	new file:   c/tlpi/t_sigwaitinfo.c 	modified:   coq/palindrome.v 	modified:   coq/parenthesis.v 	modified:   coq/sort.v 	new file:   java/JDBCExample.java 	new file:   java/JDBCExample2.java 	modified:   polyglot/Command/Command.java 	new file:   polyglot/Command/Command.scala 	new file:   polyglot/Command/command.clj 	new file:   polyglot/Command/command.cs 	new file:   polyglot/Command/command.js 	new file:   polyglot/Command/command.php 	new file:   polyglot/Command/command.py 	new file:   polyglot/Command/command.rb 	modified:   polyglot/Command/run.sh

c/tlpi/t_sigwaitinfo.c
@@ -1,0 +1,54 @@
+#define _GNU_SOURCE
+#include <string.h>
+#include <signal.h>
+#include <time.h>
+#include "tlpi_hdr.h"
+
+int
+main(int argc, char *argv[])
+{
+  int sig;
+  siginfo_t si;
+  sigset_t allSigs;
+
+  if (argc > 1 && strcmp(argv[1], "--help") == 0)
+    usageErr("%s [delay-secs]\n", argv[0]);
+
+  printf("%s: PID is %ld\n", argv[0], (long) getpid());
+
+  /* Block all signals (except SIGKILL and SIGSTOP) */
+
+  sigfillset(&allSigs);
+  if (sigprocmask(SIG_SETMASK, &allSigs, NULL) == -1)
+    errExit("sigprocmask");
+  printf("%s: signals blocked\n", argv[0]);
+
+  if (argc > 1) {     /* Delay so that signals can be sent to us */
+    printf("%s: about to delay %s seconds\n", argv[0], argv[1]);
+    sleep(getInt(argv[1], GN_GT_0, "delay-secs"));
+    printf("%s: finished delay\n", argv[0]);
+  }
+
+  for (;;) {      /* Fetch signals until SIGINT (^C) or SIGTERM */
+    sig = sigwaitinfo(&allSigs, &si);
+    if (sig == -1)
+      errExit("sigwaitinfo");
+
+    if (sig == SIGINT || sig == SIGTERM)
+      exit(EXIT_SUCCESS);
+
+    printf("got signal: %d (%s)\n", sig, strsignal(sig));
+    printf("    si_signo=%d, si_code=%d (%s), si_value=%d\n",
+        si.si_signo, si.si_code,
+        (si.si_code == SI_USER) ? "SI_USER" :
+        (si.si_code == SI_QUEUE) ? "SI_QUEUE" : "other",
+        si.si_value.sival_int);
+
+    printf("    si_pid=%ld, si_uid=%ld\n",
+        (long) si.si_pid, (long) si.si_uid);
+  }
+}
+
+
+
+
