java/JDBCExample2.java
@@ -1,0 +1,32 @@
+import java.sql.Connection;     // Connection class
+import java.sql.DriverManager;  // DriverManager class
+import java.sql.SQLException;   // SQLException class
+
+// DO NOT FORGET after compiling
+// java -cp .:/usr/share/java/postgresql-jdbc4.jar JDBCExample2
+
+public class JDBCExample2 {
+
+  // port 5432 seems to be default port for postgresql. Its inclusion in url
+  // seems to be optional here. It is not clear why connection seems to be
+  // succesful, regardless of ufw settings.
+  private static final String url = "jdbc:postgresql://127.0.0.1:5432/test";
+  private static final String user = "john";
+  private static final String password = "john";
+
+  public static void main(String[] args){
+    Connection conn = connect();
+  }
+
+  public static Connection connect(){
+    Connection conn = null;
+    try {
+      conn = DriverManager.getConnection(url, user, password);
+      System.out.println("Connected to PostgreSQL server succesfully.");
+    } catch (SQLException e){
+      System.out.println(e.getMessage());
+    }
+
+    return conn;
+  }
+}
