polyglot/Command/Command.scala
@@ -29,8 +29,8 @@
 // bookkeeping or modes.
 
 // This is the Command interface
-interface ICommand {          // our demo class is called 'Command'
-  public void execute();
+trait ICommand {
+  def execute() : Unit
 }
 
 // This is the Invoker class. It is akin to the remote control of an 
@@ -38,22 +38,11 @@ interface ICommand {          // our demo class is called 'Command'
 // the client perform actions through a single interface, without
 // having to worry about the various part of a system. The invoker class
 // it itself very generic and is unaware if the specifics of commands.
-class RemoteControl {
-  private final ICommand _powerOn;
-  private final ICommand _powerOff;
-  private final ICommand _volumeUp;
-  private final ICommand _volumeDown;
-  public RemoteControl(ICommand on, ICommand off, ICommand up, ICommand down){
-    this._powerOn     = on;
-    this._powerOff    = off;
-    this._volumeUp    = up;
-    this._volumeDown  = down;
-  }
-
-  public void switchPowerOn() { _powerOn.execute();   }
-  public void switchPowerOff(){ _powerOff.execute();  }
-  public void raiseVolume()   { _volumeUp.execute();  }
-  public void lowerVolume()   { _volumeDown.execute();}
+class RemoteControl(on: ICommand, off: ICommand, up: ICommand, down: ICommand){
+  def switchPowerOn()   = on.execute()
+  def switchPowerOff()  = off.execute()
+  def raiseVolume()     = up.execute()
+  def lowerVolume()     = down.execute()
 }
 
 // This is the receiver class. It is the class of objects which will perform
@@ -67,34 +56,38 @@ class RemoteControl {
 // as in general, the interface of the invoker object may have little in
 // common with those of the various receiver objects.
 class Television {
-  private int     _volume = 10;
-  private boolean _isOn = false;
-  public Television(){}
-  public void switchOn(){
+  private var _volume = 10;
+  private var _isOn   = false; 
+  
+  def switchOn(): Unit = {
     if(_isOn == false){
       _isOn = true;
-      System.out.println("Televion is now switched on");
+      println("Television is now switched on");
     }
   }
-  public void switchOff(){
+
+  def switchOff(): Unit = {
     if(_isOn){
       _isOn = false;
-      System.out.println("Television is now switched off");
+      println("Television is now switched off");
     }
   }
-  public void volumeUp(){
+
+  def volumeUp(): Unit = {
     if(_isOn && _volume < 20){
-      _volume++;
-      System.out.println("Television volume increased to " + _volume);
+      _volume += 1;
+      println("Television volume increased to " + _volume);
     }
   }
-  public void volumeDown(){
+
+  def volumeDown(): Unit = {
     if(_isOn && _volume > 0){
-      _volume--;
-      System.out.println("Television volume decreased to " + _volume);
+      _volume -= 1;
+      println("Television volume decreased to " + _volume);
     }
   }
 }
+
 
 // These are the concrete command objects. These commands have exact
 // knowledge of receiver objects as well as which methods and argument
@@ -103,60 +96,37 @@ class Television {
 // of indirection: client code will call an invoker object (menu, remote)
 // which will in turn execute a command, which will send a request to
 // to a receiver object, which will finally perform the requested action.
-class OnCommand implements ICommand {
-  private final Television _television;
-  public OnCommand(Television device){
-    _television = device;
-  }
-  public void execute(){
-    _television.switchOn();
-  }
+class OnCommand(television:Television) extends ICommand {
+  def execute() = television.switchOn()
+}
+  
+class OffCommand(television:Television) extends ICommand {
+  def execute() = television.switchOff()
 }
 
-class OffCommand implements ICommand {
-  private final Television _television;
-  public OffCommand(Television device){
-    _television = device;
-  }
-  public void execute(){
-    _television.switchOff();
-  }
+class UpCommand(television:Television) extends ICommand {
+  def execute() = television.volumeUp()
 }
 
-class UpCommand implements ICommand {
-  private final Television _television;
-  public UpCommand(Television device){
-    _television = device;
-  }
-  public void execute(){
-    _television.volumeUp();
-  }
+class DownCommand(television:Television) extends ICommand {
+  def execute() = television.volumeDown()
 }
 
-class DownCommand implements ICommand {
-  private final Television _television;
-  public DownCommand(Television device){
-    _television = device;
-  }
-  public void execute(){
-    _television.volumeDown();
-  }
-}
 
 // let's try it all out
-public class Command {
-  public static void main(String[] args){
+object Command {
+  def main(args: Array[String]){
     // our application will need some reveiver object
-    Television device = new Television();
+    val device = new Television()
     // our application will need an invoker object, which
     // in turns relies on concrete command objects:
-    ICommand on   = new OnCommand(device);  // command to switch device on
-    ICommand off  = new OffCommand(device); // command to switch device off
-    ICommand up   = new UpCommand(device);  // command to turn volume up
-    ICommand down = new DownCommand(device);// command to turn volume down
+    val on   = new OnCommand(device)  // command to switch device on
+    val off  = new OffCommand(device) // command to switch device off
+    val up   = new UpCommand(device)  // command to turn volume up
+    val down = new DownCommand(device)// command to turn volume down
     // now we are ready to create our invoker object which
     // we should think of as some sort of application menu.
-    RemoteControl menu = new RemoteControl(on, off, up, down);
+    val menu = new RemoteControl(on, off, up, down);
     // client code is now able to access the invoker object
     menu.switchPowerOn();
     menu.raiseVolume();
