polyglot/Command/command.clj
@@ -1,0 +1,177 @@
+; Command Design Pattern
+(ns command (:gen-class))
+; from https://en.wikipedia.org/wiki/Command_pattern 
+; In object-oriented programming, the command pattern is a behavioral 
+; design pattern in which an object is used to encapsulate all information 
+; needed to perform an action or trigger an event at a later time. This 
+; information includes the method name, the object that owns the method 
+; and values for the method parameters.
+;
+; Four terms always associated with the command pattern are command, 
+; receiver, invoker and client. A command object knows about receiver 
+; and calls a method of the receiver. Values for parameters of the 
+; receiver method are stored in the command. The receiver then does 
+; the work. An invoker object knows how to execute a command, and 
+; optionally does bookkeeping about the command execution. The invoker 
+; does not know anything about a concrete command, it knows only about 
+; command interface. Both an invoker object and several command objects 
+; are held by a client object. The client decides which commands to 
+; execute at which points. To execute a command, it passes the command 
+; object to the invoker object.
+;
+; Using command objects makes it easier to construct general components 
+; that need to delegate, sequence or execute method calls at a time of 
+; their choosing without the need to know the class of the method or the 
+; method parameters. Using an invoker object allows bookkeeping about 
+; command executions to be conveniently performed, as well as implementing 
+; different modes for commands, which are managed by the invoker object, 
+; without the need for the client to be aware of the existence of 
+; bookkeeping or modes.
+
+(defmulti execute :type)
+; This is the Command interface
+(def Command    ; constructor
+  (letfn
+    ; object created from data is message passing interface
+    [(this [data]
+       (fn [m]
+         (cond (= m :execute) (execute data)
+               :else (throw 
+                       (Exception. (format "Command: unknown operation %s" m))))))]
+    ;
+    ; returning single argument constructor
+    ;
+    (fn [data] (this data))))
+
+(defmethod execute ::command [data]
+  (throw (Exception. "Command::execute is abstract")))
+
+; This is the Invoker class. It is akin to the remote control of an 
+; electronic device, or a menu object within an application. It allows
+; the client perform actions through a single interface, without
+; having to worry about the various part of a system. The invoker class
+; it itself very generic and is unaware if the specifics of commands.
+(def RemoteControl  ; constructor
+  (letfn
+    ;
+    [(switchPowerOn   [data]  ((:powerOn data)    :execute))
+     (switchPowerOff  [data]  ((:powerOff data)   :execute))
+     (raiseVolume     [data]  ((:volumeUp data)   :execute))
+     (lowerVolume     [data]  ((:volumeDown data) :execute))
+     ; object created from data is message passing interface
+     (this [data]
+       (fn [m]
+         (cond (= m :switchPowerOn)   (switchPowerOn data)
+               (= m :switchPowerOff)  (switchPowerOff data)
+               (= m :raiseVolume)     (raiseVolume data)
+               (= m :lowerVolume)     (lowerVolume data)
+               :else (throw
+                       (Exception. (format "RemoteControl: unknown operation %s"
+                                           m))))))]
+    ;
+    ; returning four arguments constructor
+    ;
+    (fn [on off up down]
+      (this { :powerOn on :powerOff off :volumeUp up :volumeDown down }))))
+
+; This is the receiver class. It is the class of objects which will perform
+; the various actions. There may be sereral receiver classes comprising
+; a system, and the invoker object may invoke commands which applies
+; to many different receivers. Typically a menu will execute actions 
+; involving not just the application object, but many other sub-objects 
+; As this is a simple coding exercise with one receiver object, their
+; seems to be a correspondance between the interface of the RemoteControl
+; and that of the Televion. However, this correspondance is misleading
+; as in general, the interface of the invoker object may have little in
+; common with those of the various receiver objects.
+(def Television   ; constructor
+  (letfn
+    ;
+    [(switchOn [data]
+      (if (= @(data :isOn) false)
+        (do (dosync (ref-set (data :isOn) true))
+            (println "Television is now switched on"))))
+    ;
+    (switchOff [data]
+      (if (= @(data :isOn) true)
+        (do (dosync (ref-set (data :isOn) false))
+            (println "Television is now switched off"))))
+    ;
+    (volumeUp [data]
+      (if (and (= @(data :isOn) true) (< @(data :volume) 20))
+        (do (dosync (alter (data :volume) inc))
+            (println "Television volume increased to" @(data :volume)))))
+    ;
+    (volumeDown [data]
+      (if (and (= @(data :isOn) true) (> @(data :volume) 0))
+        (do (dosync (alter (data :volume) dec))
+            (println "Television volume decreased to" @(data :volume)))))
+    ; object created from data is message passing interface
+    (this [data]
+      (fn [m]
+        (cond (= m :switchOn)   (switchOn data)
+              (= m :switchOff)  (switchOff data)
+              (= m :volumeUp)   (volumeUp data)
+              (= m :volumeDown) (volumeDown data)
+              :else (throw
+                      (Exception. 
+                        (format "Television: unknown operation %s" m))))))]
+    ;
+    ; returning no argument constructor
+    ;
+    (fn [] (this { :isOn (ref false) :volume (ref 10) }))))
+
+
+; These are the concrete command objects. These commands have exact
+; knowledge of receiver objects as well as which methods and argument
+; should be used when issuing a request to receiver objects.
+; As can be seen, the command design pattern relies on a fair amount
+; of indirection: client code will call an invoker object (menu, remote)
+; which will in turn execute a command, which will send a request to
+; to a receiver object, which will finally perform the requested action.
+(def OnCommand
+  (fn [television]
+    (Command {:type ::on-command :television television})))
+(derive ::command ::on-command)
+(defmethod execute ::on-command [data] ((:television data) :switchOn))
+
+(def OffCommand
+  (fn [television]
+    (Command {:type ::off-command :television television})))
+(derive ::command ::off-command)
+(defmethod execute ::off-command [data] ((:television data) :switchOff))
+
+(def UpCommand
+  (fn [television]
+    (Command {:type ::up-command :television television})))
+(derive ::command ::up-command)
+(defmethod execute ::up-command [data] ((:television data) :volumeUp))
+
+(def DownCommand
+  (fn [television]
+    (Command {:type ::down-command :television television})))
+(derive ::command ::down-command)
+(defmethod execute ::down-command [data] ((:television data) :volumeDown))
+
+; let's try it all out
+(defn -main []
+  ; our application will need some reveiver object
+  (let [device  (Television)
+        ; our application will need an invoker object, which
+        ; in turns relies on concrete command objects:
+        on      (OnCommand    device) ; command to switch device on
+        off     (OffCommand   device) ; command to switch device off
+        up      (UpCommand    device) ; command to turn volume up
+        down    (DownCommand  device) ; command to turn volume down
+        ; now we are ready to create our invoker object which
+        ; we should think of as some sort of application menu.
+        menu    (RemoteControl on off up down)]
+    ; client code is now able to access the invoker object
+    (menu :switchPowerOn)
+    (menu :raiseVolume)
+    (menu :raiseVolume)
+    (menu :raiseVolume)
+    (menu :lowerVolume)
+    (menu :switchPowerOff)))
+
+;(-main)
