polyglot/Command/command.rb
@@ -1,0 +1,170 @@
+# Command Design Pattern
+
+# from https://en.wikipedia.org/wiki/Command_pattern 
+# In object-oriented programming, the command pattern is a behavioral 
+# design pattern in which an object is used to encapsulate all information 
+# needed to perform an action or trigger an event at a later time. This 
+# information includes the method name, the object that owns the method 
+# and values for the method parameters.
+#
+# Four terms always associated with the command pattern are command, 
+# receiver, invoker and client. A command object knows about receiver 
+# and calls a method of the receiver. Values for parameters of the 
+# receiver method are stored in the command. The receiver then does 
+# the work. An invoker object knows how to execute a command, and 
+# optionally does bookkeeping about the command execution. The invoker 
+# does not know anything about a concrete command, it knows only about 
+# command interface. Both an invoker object and several command objects 
+# are held by a client object. The client decides which commands to 
+# execute at which points. To execute a command, it passes the command 
+# object to the invoker object.
+#
+# Using command objects makes it easier to construct general components 
+# that need to delegate, sequence or execute method calls at a time of 
+# their choosing without the need to know the class of the method or the 
+# method parameters. Using an invoker object allows bookkeeping about 
+# command executions to be conveniently performed, as well as implementing 
+# different modes for commands, which are managed by the invoker object, 
+# without the need for the client to be aware of the existence of 
+# bookkeeping or modes.
+
+# This is the Command interface
+class Command
+  def execute() 
+    raise NotImplementedError.new "Command::execute is abstract" 
+  end
+end
+
+# This is the Invoker class. It is akin to the remote control of an 
+# electronic device, or a menu object within an application. It allows
+# the client perform actions through a single interface, without
+# having to worry about the various part of a system. The invoker class
+# it itself very generic and is unaware if the specifics of commands.
+class RemoteControl
+  def initialize(on, off, up, down)
+    @powerOn    = on 
+    @powerOff   = off
+    @volumeUp   = up
+    @volumeDown = down
+  end
+
+  def switchPowerOn()   @powerOn.execute()    end
+  def switchPowerOff()  @powerOff.execute()   end
+  def raiseVolume()     @volumeUp.execute()   end
+  def lowerVolume()     @volumeDown.execute() end
+end
+
+
+# This is the receiver class. It is the class of objects which will perform
+# the various actions. There may be sereral receiver classes comprising
+# a system, and the invoker object may invoke commands which applies
+# to many different receivers. Typically a menu will execute actions 
+# involving not just the application object, but many other sub-objects 
+# As this is a simple coding exercise with one receiver object, their
+# seems to be a correspondance between the interface of the RemoteControl
+# and that of the Televion. However, this correspondance is misleading
+# as in general, the interface of the invoker object may have little in
+# common with those of the various receiver objects.
+
+class Television
+  def initialize()
+    @volume = 10
+    @isOn = false
+  end
+
+  def switchOn()
+    if @isOn == false then
+      @isOn = true
+      puts "Television is now switched on"
+    end
+  end
+
+  def switchOff()
+    if @isOn then
+      @isOn = false
+      puts "Television is now switched off"
+    end
+  end
+
+  def volumeUp()
+    if @isOn && @volume < 20 then
+      @volume += 1
+      puts "Television volume increased to #{@volume}"
+    end
+  end
+
+  def volumeDown()
+    if @isOn && @volume > 0 then
+      @volume -= 1
+      puts "Television volume decreased to #{@volume}"
+    end
+  end
+end
+
+# These are the concrete command objects. These commands have exact
+# knowledge of receiver objects as well as which methods and argument
+# should be used when issuing a request to receiver objects.
+# As can be seen, the command design pattern relies on a fair amount
+# of indirection: client code will call an invoker object (menu, remote)
+# which will in turn execute a command, which will send a request to
+# to a receiver object, which will finally perform the requested action.
+class OnCommand < Command 
+  def initialize(television)
+    @television = television
+  end
+  def execute()
+    @television.switchOn()
+  end
+end
+
+class OffCommand < Command 
+  def initialize(television)
+    @television = television
+  end
+  def execute()
+    @television.switchOff()
+  end
+end
+
+class UpCommand < Command 
+  def initialize(television)
+    @television = television
+  end
+  def execute()
+    @television.volumeUp()
+  end
+end
+
+class DownCommand < Command 
+  def initialize(television)
+    @television = television
+  end
+  def execute()
+    @television.volumeDown()
+  end
+end
+
+# let's try it all out
+# our application will need some receiver object
+television = Television.new
+# our application will need an invoker object, which
+# in turns relies on concrete command objects:
+on    = OnCommand.new(television)   # command to switch tv on
+off   = OffCommand.new(television)  # command to switch tv on
+up    = UpCommand.new(television)   # command to switch tv on
+down  = DownCommand.new(television) # command to switch tv on
+# now we are ready to create our invoker object which
+# we should think of as some sort of application menu.
+menu = RemoteControl.new(on, off, up, down)
+# client code is now able to access the involker object
+menu.switchPowerOn()
+menu.raiseVolume()
+menu.raiseVolume()
+menu.raiseVolume()
+menu.lowerVolume()
+menu.switchPowerOff()
+
+
+
+
+
