coq/parenthesis.v
@@ -17,4 +17,53 @@ Qed.
 Lemma wp_o_head_c: forall (l1 l2:list par),
   wp l1 -> wp l2 -> wp (open::(l1++(close::l2))).
 Proof.
-  intros l1 l2. 
+  intros l1 l2 H1 H2. cut (nil++l2 = l2). intro H. rewrite <- H.
+  rewrite app_comm_cons with (x:=nil).
+  rewrite app_comm_cons with (a:=open). rewrite app_assoc.
+  apply wp_concat. apply wp_open_close. exact H1. exact H2. apply app_nil_l.
+Qed.
+
+
+Lemma wp_o_tail_c: forall (l1 l2:list par),
+  wp l1 -> wp l2 -> wp (l1 ++ (open :: (l2 ++ (close :: nil)))).
+Proof.
+  intros l1 l2 H1 H2. apply wp_concat. exact H1. apply wp_open_close. exact H2.
+Qed.
+
+Inductive bin : Set :=
+  | L : bin
+  | N : bin -> bin -> bin.
+
+Fixpoint bin2string (t:bin) : list par :=
+  match t with
+    | L     => nil
+    | N u v => open :: ((bin2string u) ++ (close :: (bin2string v)))
+  end.
+ 
+Lemma wp_bin2string: forall t:bin, wp (bin2string t).
+Proof.
+  intro t. elim t. simpl. apply wp_nil. clear t.
+  intros t1 H1 t2 H2. simpl. apply wp_o_head_c. exact H1. exact H2.
+Qed.
+
+
+Fixpoint bin2string' (t:bin) : list par :=
+  match t with
+    | L     => nil
+    | N u v => (bin2string' u) ++ (open :: ((bin2string' v) ++ (close :: nil)))
+  end.
+ 
+
+Lemma wp_bin2string': forall t:bin, wp (bin2string' t).
+Proof.
+  intro t. elim t. simpl. apply wp_nil. clear t.
+  intros t1 H1 t2 H2. simpl. apply wp_o_tail_c. exact H1. exact H2.
+Qed.
+
+
+
+
+
+
+
+
