polyglot/Command/run.sh
@@ -1,11 +1,70 @@
 #!/bin/sh
 
-
-
 echo '\nThis is Java ...'
 javac Command.java 
 START=$(date +%s%N)
 java Command 
+END=$(date +%s%N)
+DIFF=$(( $END - $START ))
+echo "It took $(( $DIFF / 1000000 )) ms"
+rm *.class
+
+
+echo '\nThis is C# ...'
+mcs command.cs 
+START=$(date +%s%N)
+mono command.exe 
+END=$(date +%s%N)
+DIFF=$(( $END - $START ))
+echo "It took $(( $DIFF / 1000000 )) ms"
+rm command.exe
+
+
+echo '\nThis is Scala ...'
+env JAVA_HOME=/usr/lib/jvm/java-7-openjdk-amd64 scalac Command.scala
+START=$(date +%s%N)
+scala Command 
+END=$(date +%s%N)
+DIFF=$(( $END - $START ))
+echo "It took $(( $DIFF / 1000000 )) ms"
+rm *.class
+
+
+echo '\nThis is Python ...'
+START=$(date +%s%N)
+python3 command.py
+END=$(date +%s%N)
+DIFF=$(( $END - $START ))
+echo "It took $(( $DIFF / 1000000 )) ms"
+
+
+echo '\nThis is Ruby ...'
+START=$(date +%s%N)
+ruby command.rb
+END=$(date +%s%N)
+DIFF=$(( $END - $START ))
+echo "It took $(( $DIFF / 1000000 )) ms"
+
+
+echo '\nThis is JavaScript ...'
+START=$(date +%s%N)
+js command.js
+END=$(date +%s%N)
+DIFF=$(( $END - $START ))
+echo "It took $(( $DIFF / 1000000 )) ms"
+
+echo '\nThis is PHP ...'
+START=$(date +%s%N)
+php command.php
+END=$(date +%s%N)
+DIFF=$(( $END - $START ))
+echo "It took $(( $DIFF / 1000000 )) ms"
+
+
+echo '\nThis is Clojure ...'
+clojurec command 1> /dev/null 
+START=$(date +%s%N)
+java -cp .:/usr/share/java/clojure-1.6.0.jar command
 END=$(date +%s%N)
 DIFF=$(( $END - $START ))
 echo "It took $(( $DIFF / 1000000 )) ms"
